doc/simple/coq/Subst.v
@@ -46,7 +46,7 @@ Qed.
 Lemma ctxsubst_inv_typvar : forall H G I' x t1 t2,
     ACpltCtxSubstCtx (H & x ~ AC_Typ t1) (G & x ~ AC_Typ t2) I' ->
     exists I t1', (I' = I & x ~ DC_Typ t1' /\
-    CompleteCtx H /\ ACpltCtxSubstCtx H G I /\ ACtxSubst H t1 = ACtxSubst H t2 /\
+    CompleteCtx H /\ ACpltCtxSubstCtx H G I /\ ACtxTSubst H t1 = ACtxTSubst H t2 /\
     ACpltCtxSubst H t1 t1').
 Proof.
   intros. inversions H0.
@@ -63,24 +63,22 @@ Proof.
   destruct (eq_push_inv H2) as [? [? ?]]. false.
 Qed.
 
-Lemma ctxsubst_inv_bndvar : forall H G I' x s1 s2 t1 t2,
-    ACpltCtxSubstCtx (H & x ~ AC_Bnd s1 t1) (G & x ~ AC_Bnd s2 t2) I' ->
-    exists I s1' t1', (I' = I & x ~ DC_Bnd s1' t1' /\
-      CompleteCtx H /\ ACpltCtxSubstCtx H G I /\
-      ACtxSubst H t1 = ACtxSubst H t2 /\
-      ACtxTSubst H s1 = ACtxTSubst H s2 /\
-      ACpltCtxSubst H t1 t1' /\
-      ACpltCtxTSubst H s1 s1').
+Lemma ctxsubst_inv_tvar : forall H G I' x,
+    ACpltCtxSubstCtx (H & x ~ AC_TVar) (G & x ~ AC_TVar) I' ->
+    exists I, (I' = I & x ~ DC_TVar /\
+      CompleteCtx H /\ ACpltCtxSubstCtx H G I).
 Proof.
   intros. inversions H0.
   false. apply* empty_push_inv.
   destruct (eq_push_inv H2) as [? [? ?]]. false.
-  destruct (eq_push_inv H2) as [? [? ?]]. false.
-  exists I s1' t1'.
+  exists I.
   destruct (eq_push_inv H2) as [? [? ?]]; subst.
   destruct (eq_push_inv H3) as [? [? ?]]; subst.
-  inversions H10; inversions H1.
-  split*.
+  inversions H8; inversions H1.
+  destruct (eq_push_inv H2) as [? [? ?]]; subst.
+  destruct (eq_push_inv H3) as [? [? ?]]; subst.
+  exists I.
+  auto.
   destruct (eq_push_inv H2) as [? [? ?]]. false.
   destruct (eq_push_inv H2) as [? [? ?]]. false.
   destruct (eq_push_inv H2) as [? [? ?]]. false.
@@ -107,11 +105,11 @@ Proof.
   lets: IHsub H3.
   destruct H4 as (v2 & bd2). exists~ v2.
 
-  destruct (eq_var_dec x x0).
-  subst. exists~ (AC_Bnd s1 t1).
+  destruct (eq_var_dec x a).
+  subst. exists~ AC_TVar.
   lets: binds_push_neq_inv bd n.
-  lets: IHsub H5.
-  destruct H6 as (v2 & bd2). exists~ v2.
+  lets: IHsub H1.
+  destruct H2 as (v2 & bd2). exists~ v2.
 
   destruct (eq_var_dec x a).
   subst. exists~ (AC_Solved_EVar t).
@@ -161,7 +159,7 @@ Lemma ctxsubst_inv_ssevar : forall H G I t1 t2 a,
     ACpltCtxSubstCtx (H & a ~ AC_Solved_EVar t1) (G & a ~ AC_Solved_EVar t2) I ->
     CompleteCtx H /\
     ACpltCtxSubstCtx H G I /\
-    ACtxSubst H t1 = ACtxSubst H t2.
+    ACtxTSubst H t1 = ACtxTSubst H t2.
 Proof.
   intros. inversions H0.
   false. apply* empty_push_inv.
@@ -237,51 +235,30 @@ Proof.
   destruct (ok_middle_eq H6 eq_refl H1 eq_refl H2) as [? [? ?]].
   inversions H8; subst.
   apply* IHHyp1.
-  rewrite -> (IHHyp1_1 d0 H2).
-  rewrite -> (IHHyp1_2 d3 H4).
-  auto.
+  f_equal *. lets: (IHHyp1_1 (DT_Expr d0) H2). inversion~ H.
+  lets: (IHHyp1_2 (DT_Expr d3) H4). inversion~ H0.
 
   DeclInfra.pick_fresh y.
-  assert (d ^ y = d0 ^ y). apply* H0.
-  apply open_var_inj in H1; auto.
+  assert (DT_Expr (d ^ y) = DT_Expr (d0 ^ y)). apply* H0. inversion~ H1.
+  apply dopen_var_inj in H4; auto.
   subst*.
 
   rewrite -> (IHHyp1 d0 H4).
   DeclInfra.pick_fresh y.
-  assert (d2 ^ y = d3 ^ y). apply* H0.
-  apply open_var_inj in H1; auto.
+  assert (d2 ^' y = d3 ^' y). apply* H0.
+  apply dopent_var_inj in H1; auto.
   subst*.
 
-  rewrite -> (IHHyp1 d0 H4).
-  DeclInfra.pick_fresh y.
-  assert (d2 ^ y = d3 ^ y). apply* H0.
-  apply open_var_inj in H1; auto.
-  subst*.
-
-  rewrite -> (IHHyp1 d0 H1).
-  auto.
-  rewrite -> (IHHyp1 d0 H1).
-  auto.
-  rewrite -> (IHHyp1_1 d0 H2).
+  lets: (IHHyp1 (DT_Expr d0) H1). inversion~ H.
+  lets: (IHHyp1 (DT_Expr d0) H1). inversion~ H.
+  lets: (IHHyp1_1 (DT_Expr d0) H2). inversion~ H.
   rewrite -> (IHHyp1_2 d3 H4).
   auto.
-Qed.
-
-Lemma cplt_ctxtsubst_eq : forall G t1 t2 t2',
-    ACpltCtxTSubst G t1 t2 ->
-    ACpltCtxTSubst G t1 t2' ->
-    t2 = t2'.
-Proof.
-  introv Hyp1. gen t2'. inductions Hyp1; introv Hyp2; inversions Hyp2; auto.
 
   DeclInfra.pick_fresh y.
-  assert (s2 ^' y = s3 ^' y). apply* H0.
-  apply opent_var_inj in H1; auto.
+  assert (s2 ^%' y = s3 ^%' y). apply* H0.
+  apply dtopent_var_inj in H1; auto.
   subst*.
-
-  assert (t2 = t3).
-  apply* cplt_ctxsubst_eq.
-  rewrite* H0.
 Qed.
 
 Lemma stable_cplt_env_eq : forall G H I J,
@@ -306,12 +283,10 @@ Proof.
   rewrite e.
   rewrite e0.
   auto.
-  destruct (ctxsubst_inv_bndvar H5) as [I1' [s1' [t1' [? [? [? [? [? [? ?]]]]]]]]].
-  destruct (ctxsubst_inv_bndvar H6) as [I2' [s2' [t2' [? [? [? [? [? [? ?]]]]]]]]].
-  pose (IHExtCtx I1' H9 I2' H16).
-  pose (cplt_ctxsubst_eq H12 H19).
-  pose (cplt_ctxtsubst_eq H13 H20).
-  rewrite H7. rewrite H14. rewrite e; rewrite e0; rewrite e1. auto.
+  destruct (ctxsubst_inv_tvar H3) as [I1' [? [? ?]]].
+  destruct (ctxsubst_inv_tvar H4) as [I2' [? [? ?]]].
+  pose (IHExtCtx I1' H7 I2' H10).
+  rewrite H5. rewrite H8. rewrite e. auto.
   false. pose (ctxsubst_inv_uuevar H3). auto.
   destruct (ctxsubst_inv_ssevar H4) as [? [? ?]].
   destruct (ctxsubst_inv_ssevar H5) as [? [? ?]].
@@ -394,9 +369,9 @@ Proof.
   false complete_contains_unsolved comp neq.
 Qed.
 
-Lemma complete_add_bnd: forall G x t e,
+Lemma complete_add_tvar: forall G x,
     CompleteCtx G ->
-    CompleteCtx (G & x ~ AC_Bnd t e).
+    CompleteCtx (G & x ~ AC_TVar).
 Proof.
   introv comp.
   unfold CompleteCtx.
@@ -442,7 +417,7 @@ Proof.
   rewrite concat_assoc in okgh. apply* ok_concat_inv_l.
 
   rewrite concat_assoc.
-  apply~ complete_add_bnd.
+  apply~ complete_add_tvar.
   apply~ IHenv.
   apply complete_part_left in comp_h. auto. apply* ok_concat_inv_r.
   rewrite concat_assoc in okgh. apply* ok_concat_inv_l.
@@ -457,31 +432,27 @@ Proof.
   rewrite concat_assoc in okgh. apply* ok_concat_inv_l.
 Qed.
 
-
 Lemma eq_aexpr_dec : forall (T T' : AExpr),
+  sumbool (T = T') (T <> T')
+with eq_atype_dec : forall (T T' : AType),
   sumbool (T = T') (T <> T').
 Proof.
   decide equality.
   decide equality.
   apply* eq_var_dec.
-  apply* eq_var_dec.
-Qed.
-
-Lemma eq_atype_dec : forall (T T' : AType),
-  sumbool (T = T') (T <> T').
 Proof.
   decide equality.
-  apply* eq_aexpr_dec.
+  decide equality.
+  apply* eq_var_dec.
+  apply* eq_var_dec.
 Qed.
 
 Lemma eq_actx_dec : forall (T T' : ACtxT),
   sumbool (T = T') (T <> T').
 Proof.
   decide equality.
-  apply* eq_aexpr_dec.
-  apply* eq_aexpr_dec.
   apply* eq_atype_dec.
-  apply* eq_aexpr_dec.
+  apply* eq_atype_dec.
 Qed.
   
 Lemma cplt_ctx_weaken : forall G x v,
@@ -514,17 +485,13 @@ Proof.
   subst. auto.
 Qed.   
 
-
-
-
 Lemma ctxsubst_fvar_eq : forall G x v,
     ok G ->
-    (forall a1 a2, v <> AC_Bnd a1 a2) ->
     (forall a, v <> AC_Solved_EVar a) ->
     (binds x v G \/ x # G) ->
     ACtxSubst G (AE_FVar x) = AE_FVar x.
 Proof.
-  introv H NBnd NEvar H1. inductions H.
+  introv H NEvar H1. inductions H.
   rewrite* subst_empty_env.
   inductions v0.
   rewrite~ subst_add_var.
@@ -543,16 +510,13 @@ Proof.
   apply* IHok.
   apply* IHok.
 
-  rewrite~ subst_add_bndvar.
+  rewrite~ subst_add_tvar.
   destruct H1 as [Bnd | Frh].
   destruct (binds_concat_inv Bnd) as [Bnd1 | [NIn Bnd1]].
-  destruct (binds_single_inv Bnd1) as [Eq1 Eq2].
-  false. simpl. case_var~.
-  rewrite dom_single in NIn.
-  false. apply* notin_same.
-  simpl. case_var~.
-  false. rewrite dom_push in Frh.
-  apply* notin_same.
+  destruct (binds_single_inv Bnd1) as [Eq1 Eq2]; subst.
+  apply* IHok.
+  apply* IHok.
+  apply* IHok.
 
   rewrite~ subst_add_evar.
   destruct H1 as [Bnd | Frh].
@@ -566,23 +530,20 @@ Proof.
   destruct H1 as [Bnd | Frh].
   destruct (binds_concat_inv Bnd) as [Bnd1 | [NIn Bnd1]].
   destruct (binds_single_inv Bnd1) as [Eq1 Eq2].
-  false. simpl. case_var~.
-  rewrite dom_single in NIn.
-  false. apply* notin_same.
-  simpl. case_var~.
-  false. rewrite dom_push in Frh.
-  apply* notin_same.
+  false.
+  apply* IHok.
+  apply* IHok.
 Qed.
 
 Lemma ctxsubst_evar_eq : forall G x,
     ok G ->
     (binds x AC_Unsolved_EVar G \/ x # G) ->
-    ACtxSubst G (AE_EVar x) = AE_EVar x.
+    ACtxTSubst G (AT_EVar x) = AT_EVar x.
 Proof.
   introv H H1. inductions H.
-  rewrite* subst_empty_env.
+  rewrite* tsubst_empty_env.
   inductions v.
-  rewrite~ subst_add_var.
+  rewrite~ tsubst_add_var.
   destruct H1 as [Bnd | Frh].
   destruct (binds_concat_inv Bnd) as [Bnd1 | [NIn Bnd1]].
   destruct (binds_single_inv Bnd1) as [Eq1 Eq2]; subst.
@@ -590,7 +551,7 @@ Proof.
   apply* IHok.
   apply* IHok.
 
-  rewrite~ subst_add_typvar.
+  rewrite~ tsubst_add_typvar.
   destruct H1 as [Bnd | Frh].
   destruct (binds_concat_inv Bnd) as [Bnd1 | [NIn Bnd1]].
   destruct (binds_single_inv Bnd1) as [Eq1 Eq2]; subst.
@@ -598,18 +559,7 @@ Proof.
   apply* IHok.
   apply* IHok.
 
-  rewrite~ subst_add_bndvar.
-  destruct H1 as [Bnd | Frh].
-  destruct (binds_concat_inv Bnd) as [Bnd1 | [NIn Bnd1]].
-  destruct (binds_single_inv Bnd1) as [Eq1 Eq2].
-  false. simpl. case_var~.
-  rewrite dom_single in NIn.
-  false. apply* notin_same.
-  simpl. case_var~.
-  false. rewrite dom_push in Frh.
-  apply* notin_same.
-
-  rewrite~ subst_add_evar.
+  rewrite~ tsubst_add_tvar.
   destruct H1 as [Bnd | Frh].
   destruct (binds_concat_inv Bnd) as [Bnd1 | [NIn Bnd1]].
   destruct (binds_single_inv Bnd1) as [Eq1 Eq2]; subst.
@@ -617,7 +567,15 @@ Proof.
   apply* IHok.
   apply* IHok.
 
-  rewrite~ subst_add_solved_evar.
+  rewrite~ tsubst_add_evar.
+  destruct H1 as [Bnd | Frh].
+  destruct (binds_concat_inv Bnd) as [Bnd1 | [NIn Bnd1]].
+  destruct (binds_single_inv Bnd1) as [Eq1 Eq2]; subst.
+  apply* IHok.
+  apply* IHok.
+  apply* IHok.
+
+  rewrite~ tsubst_add_solved_evar.
   destruct H1 as [Bnd | Frh].
   destruct (binds_concat_inv Bnd) as [Bnd1 | [NIn Bnd1]].
   destruct (binds_single_inv Bnd1) as [Eq1 Eq2].
@@ -629,101 +587,218 @@ Proof.
   apply* notin_same.
 Qed.
 
-Lemma ctxsubst_awterm : forall G t,
+Lemma ctxsubst_tvar_eq : forall G x,
     ok G ->
-    AWTerm G t ->
-    AWTerm G (ACtxSubst G t).
+    (binds x AC_TVar G \/ x # G) ->
+    ACtxTSubst G (AT_TFVar x) = AT_TFVar x.
 Proof.
-  introv Ok Hyp. 
-  inductions Hyp.
-  assert (ACtxSubst G (AE_FVar x) = AE_FVar x).
-  apply* ctxsubst_fvar_eq. 
-  unfold not; intros. inversions H0.
-  unfold not; intros. inversions H0.
-  rewrite H0.
-  apply* AWTerm_Var.
-  
-  assert (ACtxSubst G (AE_FVar x) = AE_FVar x).
-  apply* ctxsubst_fvar_eq.
-  unfold not; intros. inversions H0.
-  unfold not; intros. inversions H0.
-  rewrite H0.
-  apply* AWTerm_TypVar.
-  
-  inductions Ok.
-  false. apply* binds_empty_inv.
+  introv H H1. inductions H.
+  rewrite* tsubst_empty_env.
   inductions v.
-  rewrite~ subst_add_var.
-  destruct (binds_concat_inv H0) as [Bnd1 | [NIn Bnd1]].
+  rewrite~ tsubst_add_var.
+  destruct H1 as [Bnd | Frh].
+  destruct (binds_concat_inv Bnd) as [Bnd1 | [NIn Bnd1]].
+  destruct (binds_single_inv Bnd1) as [Eq1 Eq2]; subst.
+  apply* IHok.
+  apply* IHok.
+  apply* IHok.
+
+  rewrite~ tsubst_add_typvar.
+  destruct H1 as [Bnd | Frh].
+  destruct (binds_concat_inv Bnd) as [Bnd1 | [NIn Bnd1]].
+  destruct (binds_single_inv Bnd1) as [Eq1 Eq2]; subst.
+  apply* IHok.
+  apply* IHok.
+  apply* IHok.
+
+  rewrite~ tsubst_add_tvar.
+  destruct H1 as [Bnd | Frh].
+  destruct (binds_concat_inv Bnd) as [Bnd1 | [NIn Bnd1]].
+  destruct (binds_single_inv Bnd1) as [Eq1 Eq2]; subst.
+  apply* IHok.
+  apply* IHok.
+  apply* IHok.
+
+  rewrite~ tsubst_add_evar.
+  destruct H1 as [Bnd | Frh].
+  destruct (binds_concat_inv Bnd) as [Bnd1 | [NIn Bnd1]].
+  destruct (binds_single_inv Bnd1) as [Eq1 Eq2]; subst.
+  apply* IHok.
+  apply* IHok.
+  apply* IHok.
+
+  rewrite~ tsubst_add_solved_evar.
+  destruct H1 as [Bnd | Frh].
+  destruct (binds_concat_inv Bnd) as [Bnd1 | [NIn Bnd1]].
   destruct (binds_single_inv Bnd1) as [Eq1 Eq2].
-  false. apply* awterm_weaken.
-  rewrite~ subst_add_typvar.
-  destruct (binds_concat_inv H0) as [Bnd1 | [NIn Bnd1]].
-  destruct (binds_single_inv Bnd1) as [Eq1 Eq2].
-  false. apply* awterm_weaken.
-  rewrite~ subst_add_bndvar.
-  destruct (binds_concat_inv H0) as [Bnd1 | [NIn Bnd1]].
-  destruct (binds_single_inv Bnd1) as [Eq1 Eq2].
-  inversions Eq2.
-  simpl. case_var~.
-  apply* awterm_weaken.
-  (* FIXME: AWTerm E (ACtxSubst E a0) *) admit.
-  simpl. case_var~.
+  false. simpl. case_var~.
   rewrite dom_single in NIn.
   false. apply* notin_same.
-  apply* awterm_weaken.
-  rewrite~ subst_add_evar.
-  destruct (binds_concat_inv H0) as [Bnd1 | [NIn Bnd1]].
-  destruct (binds_single_inv Bnd1) as [Eq1 Eq2].
-  false. apply* awterm_weaken.
-  rewrite~ subst_add_solved_evar.
-  destruct (binds_concat_inv H0) as [Bnd1 | [NIn Bnd1]].
-  destruct (binds_single_inv Bnd1) as [Eq1 Eq2].
-  false. simpl. case_var~. false.
-  rewrite dom_single in NIn.
-  false. apply* notin_same.
-  apply* awterm_weaken.
-
-  assert (ACtxSubst G (AE_EVar a) = AE_EVar a).
-  apply* ctxsubst_evar_eq.
-  unfold not; intros.
-  rewrite H0.
-  apply* AWTerm_EVar.
-
-  inductions Ok.
-  false. apply* binds_empty_inv.
-  inductions v.
-  rewrite~ subst_add_var.
-  destruct (binds_concat_inv H0) as [Bnd1 | [NIn Bnd1]].
-  destruct (binds_single_inv Bnd1) as [Eq1 Eq2].
-  false. apply* awterm_weaken.
-  rewrite~ subst_add_typvar.
-  destruct (binds_concat_inv H0) as [Bnd1 | [NIn Bnd1]].
-  destruct (binds_single_inv Bnd1) as [Eq1 Eq2].
-  false. apply* awterm_weaken.
-  rewrite~ subst_add_bndvar.
-  destruct (binds_concat_inv H0) as [Bnd1 | [NIn Bnd1]].
-  destruct (binds_single_inv Bnd1) as [Eq1 Eq2].
-  false. simpl. case_var~. false.
-  rewrite dom_single in NIn.
-  false. apply* notin_same.
-  apply* awterm_weaken.
-  rewrite~ subst_add_evar.
-  destruct (binds_concat_inv H0) as [Bnd1 | [NIn Bnd1]].
-  destruct (binds_single_inv Bnd1) as [Eq1 Eq2].
-  false. apply* awterm_weaken.
-  rewrite~ subst_add_solved_evar.
-  destruct (binds_concat_inv H0) as [Bnd1 | [NIn Bnd1]].
-  destruct (binds_single_inv Bnd1) as [Eq1 Eq2].
-  inversions Eq2.
   simpl. case_var~.
-  apply* awterm_weaken.
-  (* FIXME: AWTerm E (ACtxSubst E a) *) admit.
-  simpl. case_var~.
-  rewrite dom_single in NIn.
-  false. apply* notin_same.
-  apply* awterm_weaken.
+  false. rewrite dom_push in Frh.
+  apply* notin_same.
+Qed.
 
-  rewrite~ subst_star.
-Admitted.
+Hint Resolve awf_is_ok.
 
+(* THIS SHOULD BE PROVED BY INDUCTION ON LENGTH *)
+(* Lemma ctxsubst_awterm : forall G t, *)
+(*     AWf G -> *)
+(*     AWTermT G t -> *)
+(*     AWTermT G (ACtxTSubst G t). *)
+(* Proof. *)
+(*   introv Ok Hyp.  *)
+(*   inductions Hyp. *)
+(*   assert (ACtxTSubst G (AT_Expr (AE_FVar x)) = AT_Expr (AE_FVar x)). *)
+(*   rewrite* actxtsubst_expr. f_equal ~. *)
+(*   apply* ctxsubst_fvar_eq.  *)
+(*   unfold not; intros. inversions H0. *)
+(*   unfold not; intros. inversions H0. *)
+(*   rewrite H2. rewrite H2. *)
+(*   apply* AWTermT_Var. *)
+  
+(*   assert (ACtxTSubst G (AT_Expr (AE_FVar x)) = AT_Expr (AE_FVar x)). *)
+(*   rewrite* actxtsubst_expr. f_equal ~. *)
+(*   apply* ctxsubst_fvar_eq. *)
+(*   unfold not; intros. inversions H0. *)
+(*   rewrite H0. *)
+(*   apply* AWTermT_TypVar. *)
+
+(*   rewrite tsubst_star. *)
+(*   apply AWTermT_Star. *)
+
+(*   rewrite actxtsubst_expr in *. *)
+(*   rewrite actxsubst_app. *)
+(*   apply* AWTermT_App. *)
+
+(*   rewrite actxtsubst_expr in *. *)
+(*   rewrite actxsubst_lam. *)
+(*   apply AWTermT_Lam with (L \u dom G). *)
+(*   intros y notiny. *)
+(*   assert (AWf (G & y ~ AC_Var)). apply* AWf_Var. *)
+(*   assert (y \notin L) by auto_star. *)
+(*   lets: H0 H2 H1. *)
+(*   rewrite actxtsubst_expr in H3. *)
+(*   rewrite subst_add_var in H3. *)
+(*   admit. *)
+
+(*   rewrite actxtsubst_expr in *. *)
+(*   rewrite actxsubst_pi. *)
+(*   apply AWTermT_Pi with (L \u dom G). *)
+(*   apply* IHHyp. *)
+(*   intros y notiny. *)
+(*   assert (AWf (G & y ~ AC_Var)). apply* AWf_Var. *)
+(*   assert (y \notin L) by auto_star. *)
+(*   lets: H0 H2 H1. *)
+(*   rewrite tsubst_add_var in H3. *)
+(*   admit. *)
+
+(*   rewrite actxtsubst_expr in *. *)
+(*   rewrite actxsubst_castup. *)
+(*   apply AWTermT_CastUp. *)
+(*   apply* IHHyp. *)
+
+(*   rewrite actxtsubst_expr in *. *)
+(*   rewrite actxsubst_castdn. *)
+(*   apply AWTermT_CastDn. *)
+(*   apply* IHHyp. *)
+
+(*   rewrite actxtsubst_expr in *. *)
+(*   rewrite actxsubst_ann. *)
+(*   apply AWTermT_Ann. *)
+(*   apply* IHHyp1. apply* IHHyp2. *)
+
+(*   rewrite actxtsubst_expr in *. *)
+(*   rewrite actxsubst_forall. *)
+(*   apply AWTermT_Forall with (L \u dom G). *)
+(*   intros y notiny. *)
+(*   assert (AWf (G & y ~ AC_TVar)). apply* AWf_TVar. *)
+(*   assert (y \notin L) by auto_star. *)
+(*   lets: H0 H2 H1. *)
+(*   rewrite tsubst_add_tvar in H3. *)
+(*   admit. *)
+
+(*   rewrite* ctxsubst_tvar_eq. *)
+(*   rewrite* ctxsubst_evar_eq. *)
+
+(*   intros y notiny. *)
+(*   assert (ok (G & y ~ AC_Var)). apply* ok_push. *)
+(*   assert (y \notin L) by auto_star. *)
+(*   lets: H0 H2 H1. *)
+(*   rewrite tsubst_add_var in H3. *)
+(*   admit. *)
+
+(*   inductions Ok. *)
+(*   false. apply* binds_empty_inv. *)
+(*   inductions v. *)
+(*   rewrite~ subst_add_var. *)
+(*   destruct (binds_concat_inv H0) as [Bnd1 | [NIn Bnd1]]. *)
+(*   destruct (binds_single_inv Bnd1) as [Eq1 Eq2]. *)
+(*   false. apply* awterm_weaken. *)
+(*   rewrite~ subst_add_typvar. *)
+(*   destruct (binds_concat_inv H0) as [Bnd1 | [NIn Bnd1]]. *)
+(*   destruct (binds_single_inv Bnd1) as [Eq1 Eq2]. *)
+(*   false. apply* awterm_weaken. *)
+(*   rewrite~ subst_add_bndvar. *)
+(*   destruct (binds_concat_inv H0) as [Bnd1 | [NIn Bnd1]]. *)
+(*   destruct (binds_single_inv Bnd1) as [Eq1 Eq2]. *)
+(*   inversions Eq2. *)
+(*   simpl. case_var~. *)
+(*   apply* awterm_weaken. *)
+(*   (* FIXME: AWTerm E (ACtxSubst E a0) *) admit. *)
+(*   simpl. case_var~. *)
+(*   rewrite dom_single in NIn. *)
+(*   false. apply* notin_same. *)
+(*   apply* awterm_weaken. *)
+(*   rewrite~ subst_add_evar. *)
+(*   destruct (binds_concat_inv H0) as [Bnd1 | [NIn Bnd1]]. *)
+(*   destruct (binds_single_inv Bnd1) as [Eq1 Eq2]. *)
+(*   false. apply* awterm_weaken. *)
+(*   rewrite~ subst_add_solved_evar. *)
+(*   destruct (binds_concat_inv H0) as [Bnd1 | [NIn Bnd1]]. *)
+(*   destruct (binds_single_inv Bnd1) as [Eq1 Eq2]. *)
+(*   false. simpl. case_var~. false. *)
+(*   rewrite dom_single in NIn. *)
+(*   false. apply* notin_same. *)
+(*   apply* awterm_weaken. *)
+
+(*   assert (ACtxSubst G (AE_EVar a) = AE_EVar a). *)
+(*   apply* ctxsubst_evar_eq. *)
+(*   unfold not; intros. *)
+(*   rewrite H0. *)
+(*   apply* AWTerm_EVar. *)
+(*  false. apply* binds_empty_inv. *)
+(*   inductions v. *)
+(*   rewrite~ subst_add_var. *)
+(*   destruct (binds_concat_inv H0) as [Bnd1 | [NIn Bnd1]]. *)
+(*   destruct (binds_single_inv Bnd1) as [Eq1 Eq2]. *)
+(*   false. apply* awterm_weaken. *)
+(*   rewrite~ subst_add_typvar. *)
+(*   destruct (binds_concat_inv H0) as [Bnd1 | [NIn Bnd1]]. *)
+(*   destruct (binds_single_inv Bnd1) as [Eq1 Eq2]. *)
+(*   false. apply* awterm_weaken. *)
+(*   rewrite~ subst_add_bndvar. *)
+(*   destruct (binds_concat_inv H0) as [Bnd1 | [NIn Bnd1]]. *)
+(*   destruct (binds_single_inv Bnd1) as [Eq1 Eq2]. *)
+(*   false. simpl. case_var~. false. *)
+(*   rewrite dom_single in NIn. *)
+(*   false. apply* notin_same. *)
+(*   apply* awterm_weaken. *)
+(*   rewrite~ subst_add_evar. *)
+(*   destruct (binds_concat_inv H0) as [Bnd1 | [NIn Bnd1]]. *)
+(*   destruct (binds_single_inv Bnd1) as [Eq1 Eq2]. *)
+(*   false. apply* awterm_weaken. *)
+(*   rewrite~ subst_add_solved_evar. *)
+(*   destruct (binds_concat_inv H0) as [Bnd1 | [NIn Bnd1]]. *)
+(*   destruct (binds_single_inv Bnd1) as [Eq1 Eq2]. *)
+(*   inversions Eq2. *)
+(*   simpl. case_var~. *)
+(*   apply* awterm_weaken. *)
+(*   (* FIXME: AWTerm E (ACtxSubst E a) *) admit. *)
+(*   simpl. case_var~. *)
+(*   rewrite dom_single in NIn. *)
+(*   false. apply* notin_same. *)
+(*   apply* awterm_weaken. *)
+
+(*   rewrite~ subst_star. *)
+(* Admitted. *)
